TheologExercises2026/Exercises/Exercise04.lean
@@ -1,0 +1,46 @@
+import TheologExercises2026.Exercises.Exercise03
+
+def HornFormula (Atom : Type u) := List (HornClause Atom)
+
+instance [BEq Atom] (H : HornFormula Atom) : Decidable (H = []) := List.instDecidableEqNil H
+
+instance [BEq Atom] : BEq (HornClause Atom) where
+beq := fun C1 C2 => C1.head == C2.head && C1.body == C2.body
+
+instance [BEq Atom] : BEq (HornFormula Atom) where
+beq := fun H1 H2 => List.beq H1 H2
+
+variable {Atom : Type u}
+
+def Formula.conjunction_from_list : List (Formula Atom) -> Formula Atom
+| .nil => .top
+| .cons hd tl => match tl with
+  | .nil => hd
+  | .cons hd' tl => .and hd (conjunction_from_list (hd'::tl))
+
+namespace HornFormula
+
+def toFormula (H : HornFormula Atom) : Formula Atom :=
+  Formula.list_to_formula (H.map (fun C => C.toFormula))
+
+theorem eval_toFormula_eq (H : HornFormula Atom) (v : Valuation Atom) : v.eval H.toFormula = (H.map (·.toFormula)).all v.eval := by
+  unfold toFormula
+  simp
+
+instance : Membership (HornClause Atom) (HornFormula Atom) := List.instMembership
+
+theorem unsat_iff_contains_empty [BEq Atom] (H : HornFormula Atom) : HornClause.empty ∈ H -> H.toFormula.unsatisfiable := by
+  intro empty_mem
+  unfold Formula.unsatisfiable
+  intro contra
+  unfold Formula.satisfiable at contra
+  rcases contra with ⟨v, v_eval⟩
+  induction H with
+  | nil => contradiction
+  | cons C H' ih =>
+    rw [eval_toFormula_eq] at v_eval
+    have aux : ∀ C', C' ∈ C::H' -> v.eval C'.toFormula = true := by grind
+    have eval_empty : v.eval HornClause.empty.toFormula = true := aux HornClause.empty empty_mem
+    contradiction
+
+end HornFormula
